src/Parsers/BooleanRecognizer.v
@@ -1,0 +1,469 @@
+(** * Definition of a boolean-returning CFG parser-recognizer *)
+Require Import Coq.Lists.List Coq.Program.Program Coq.Program.Wf Coq.Arith.Wf_nat Coq.Arith.Compare_dec Coq.Classes.RelationClasses Coq.Strings.String.
+Require Import Parsers.ContextFreeGrammar Parsers.Specification.
+Require Import Common Common.ilist.
+
+Set Implicit Arguments.
+Local Open Scope string_like_scope.
+
+Section wf.
+  Section wf_prod.
+    Context A B (RA : relation A) (RB : relation B).
+
+    Definition prod_relation : relation (A * B)
+      := fun ab a'b' =>
+           RA (fst ab) (fst a'b') \/ (fst a'b' = fst ab /\ RB (snd ab) (snd a'b')).
+
+    Fixpoint well_founded_prod_relation_helper
+             a b
+             (wf_A : Acc RA a) (wf_B : well_founded RB) {struct wf_A}
+    : Acc prod_relation (a, b)
+      := match wf_A with
+           | Acc_intro fa => (fix wf_B_rec b' (wf_B' : Acc RB b') : Acc prod_relation (a, b')
+                              := Acc_intro
+                                   _
+                                   (fun ab =>
+                                      match ab as ab return prod_relation ab (a, b') -> Acc prod_relation ab with
+                                        | (a'', b'') =>
+                                          fun pf =>
+                                            match pf with
+                                              | or_introl pf'
+                                                => @well_founded_prod_relation_helper
+                                                     _ _
+                                                     (fa _ pf')
+                                                     wf_B
+                                              | or_intror (conj pfa pfb)
+                                                => match wf_B' with
+                                                     | Acc_intro fb
+                                                       => eq_rect
+                                                            _
+                                                            (fun a'' => Acc prod_relation (a'', b''))
+                                                            (wf_B_rec _ (fb _ pfb))
+                                                            _
+                                                            pfa
+                                                   end
+                                            end
+                                      end)
+                             ) b (wf_B b)
+         end.
+
+    Definition well_founded_prod_relation : well_founded RA -> well_founded RB -> well_founded prod_relation.
+    Proof.
+      intros wf_A wf_B [a b]; hnf in *.
+      apply well_founded_prod_relation_helper; auto.
+    Defined.
+  End wf_prod.
+End wf.
+
+Section recursive_descent_parser.
+  Context CharType (String : string_like CharType) (G : grammar CharType).
+  Context (productions_listT : Type)
+          (initial_productions_data : productions_listT)
+          (is_valid_productions : productions_listT -> productions CharType -> bool)
+          (remove_productions : productions_listT -> productions CharType -> productions_listT)
+          (productions_listT_R : productions_listT -> productions_listT -> Prop)
+          (remove_productions_dec : forall ls prods, is_valid_productions ls prods = true
+                                                     -> productions_listT_R (remove_productions ls prods) ls)
+          (ntl_wf : well_founded productions_listT_R).
+  Section bool.
+    Context (split_string_for_production
+             : forall (str0 : String)
+                      (prod : production CharType),
+                 list (list { str : String | Length _ str < Length _ str0 \/ str = str0 })).
+
+    Section parts.
+      Section item.
+        Context (str : String)
+                (str_matches_productions : productions CharType -> bool).
+
+        Definition parse_item (it : item CharType) : bool
+          := match it with
+               | Terminal ch => [[ ch ]] =s str
+               | NonTerminal name => str_matches_productions (Lookup G name)
+             end.
+      End item.
+
+      Section production.
+        Variable str0 : String.
+        Variable parse_productions : forall (str : String),
+                                       Length _ str < Length _ str0 \/ str = str0
+                                       -> productions CharType
+                                       -> bool.
+
+        (** To match a [production], we must match all of its items.  If the lengths do match up, we don't define the outcome. *)
+        Definition parse_production_from_split_list
+                   (strs : list { str : String | Length _ str < Length _ str0 \/ str = str0 })
+                   (prod : production CharType)
+        : bool
+          := fold_left andb
+                       (map (fun sp => parse_item (proj1_sig (fst sp))
+                                                  (parse_productions (proj2_sig (fst sp)))
+                                                  (snd sp))
+                            (combine strs prod))
+                       true.
+
+        (** To match a [production], any split of the string can match. *)
+        Definition parse_production_from_any_split_list
+                   (strs : list (list { str : String | Length _ str < Length _ str0 \/ str = str0 }))
+                   (prod : production CharType)
+        : bool
+          := fold_left orb
+                       (map (fun strs => parse_production_from_split_list strs prod)
+                            strs)
+                       false.
+
+        Definition or_transitivity {A B} `{@Transitive B R} {f : A -> B} {a0 a}
+                   (pf : R (f a) (f a0) \/ a = a0) a' (pf' : R (f a') (f a) \/ a' = a)
+        : R (f a') (f a0) \/ a' = a0.
+        Proof.
+          destruct_head or; subst;
+          first [ right; reflexivity | left; assumption | left; etransitivity; eassumption ].
+        Defined.
+
+        (** We assume the splits we are given are valid (are actually splits of the string, rather than an unrelated split) and are the same length as the given [production].  Behavior in other cases is undefined *)
+        (** We match a production if any split of the string matches that production *)
+        Definition parse_production
+                   (str : String) (pf : Length _ str < Length _ str0 \/ str = str0)
+                   (prod : production CharType)
+        : bool
+          := if (gt_dec (Datatypes.length prod) 0)
+             then (@parse_production_from_any_split_list
+                     (map (map (fun sp => exist _ (proj1_sig sp) (or_transitivity pf (proj2_sig sp))))
+                          (@split_string_for_production str prod))
+                     prod)
+             else (** 0-length production, only accept empty *)
+               (str =s Empty _).
+      End production.
+
+      Section productions.
+        Section step.
+          Variable str0 : String.
+          Variable parse_productions : forall (str : String)
+                                              (pf : Length _ str < Length _ str0 \/ str = str0),
+                                         productions CharType -> bool.
+
+          (** To parse as a given list of [production]s, we must parse as one of the [production]s. *)
+          Definition parse_productions_step (str : String) (pf : Length _ str < Length _ str0 \/ str = str0) (prods : productions CharType)
+          : bool
+            := fold_left orb
+                         (map (parse_production parse_productions pf)
+                              prods)
+                         false.
+        End step.
+
+        Section wf.
+          Definition parse_productions_or_abort (str0 str : String)
+                     (valid_list : productions_listT)
+                     (pf : Length _ str < Length _ str0 \/ str = str0)
+                     (prods : productions CharType)
+          : bool.
+          Proof.
+            revert str pf prods.
+            change str0 with (fst (pair str0 valid_list)).
+            generalize (pair str0 valid_list); clear str0 valid_list.
+            refine (@Fix (prod String productions_listT)
+                         _ (@well_founded_prod_relation
+                              String
+                              productions_listT
+                              _
+                              _
+                              (well_founded_ltof _ (Length String))
+                              ntl_wf)
+                         _ _).
+            intros [str0 valid_list] parse_productions str pf prods; simpl in *.
+            destruct (lt_dec (Length _ str) (Length _ str0)) as [pf'|pf'].
+            { (** [str] got smaller, so we reset the valid productions list *)
+              specialize (parse_productions
+                            (pair str initial_productions_data)
+                            (or_introl pf')); simpl in *.
+              exact (parse_productions_step parse_productions (or_intror eq_refl) prods). }
+            { (** [str] didn't get smaller, so we cache the fact that we've hit this productions already *)
+              case_eq (is_valid_productions valid_list prods).
+              { (** It was valid, so we can remove it *)
+                intro H'.
+                specialize (fun pf' => parse_productions
+                              (pair str0 (remove_productions valid_list prods))
+                              (or_intror (conj eq_refl pf'))); simpl in *.
+                specialize (parse_productions (remove_productions_dec H')).
+                exact (parse_productions_step parse_productions (or_intror eq_refl) prods). }
+              { (** oops, we already saw this productions in the past.  ABORT! *)
+                intro; exact false. } }
+          Defined.
+
+          Definition parse_productions (str : String) (prods : productions CharType)
+          : bool
+            := @parse_productions_or_abort str str initial_productions_data
+                                           (or_intror eq_refl) prods.
+        End wf.
+      End productions.
+    End parts.
+  End bool.
+End recursive_descent_parser.
+
+Section recursive_descent_parser_list.
+  Context {CharType} {String : string_like CharType} {G : grammar CharType}.
+  Variable (CharType_eq_dec : forall x y : CharType, {x = y} + {x <> y}).
+  Definition rdp_list_productions_listT : Type := list (productions CharType).
+  Definition rdp_list_is_valid_productions : rdp_list_productions_listT -> productions CharType -> bool
+    := fun ls nt => if in_dec (productions_dec CharType_eq_dec) nt ls then true else false.
+  Definition rdp_list_remove_productions : rdp_list_productions_listT -> productions CharType -> rdp_list_productions_listT
+    := fun ls nt =>
+         filter (fun x => if productions_dec CharType_eq_dec nt x then false else true) ls.
+  Definition rdp_list_productions_listT_R : rdp_list_productions_listT -> rdp_list_productions_listT -> Prop
+    := ltof _ (@List.length _).
+  Lemma filter_list_dec {T} f (ls : list T) : List.length (filter f ls) <= List.length ls.
+  Proof.
+    induction ls; trivial; simpl in *.
+    repeat match goal with
+             | [ |- context[if ?a then _ else _] ] => destruct a; simpl in *
+             | [ |- S _ <= S _ ] => solve [ apply Le.le_n_S; auto ]
+             | [ |- _ <= S _ ] => solve [ apply le_S; auto ]
+           end.
+  Defined.
+  Lemma rdp_list_remove_productions_dec : forall ls prods,
+                                            @rdp_list_is_valid_productions ls prods = true
+                                            -> @rdp_list_productions_listT_R (@rdp_list_remove_productions ls prods) ls.
+  Proof.
+    intros.
+    unfold rdp_list_is_valid_productions, rdp_list_productions_listT_R, rdp_list_remove_productions, ltof in *.
+    destruct (in_dec (productions_dec CharType_eq_dec) prods ls); [ | discriminate ].
+    match goal with
+      | [ H : In ?prods ?ls |- context[filter ?f ?ls] ]
+        => assert (~In prods (filter f ls))
+    end.
+    { intro H'.
+      apply filter_In in H'.
+      destruct H' as [? H'].
+      destruct (productions_dec CharType_eq_dec prods prods); congruence. }
+    { match goal with
+        | [ |- context[filter ?f ?ls] ] => generalize dependent f; intros
+      end.
+      induction ls; simpl in *; try congruence.
+      repeat match goal with
+               | [ |- context[if ?x then _ else _] ] => destruct x; simpl in *
+               | [ H : _ \/ _ |- _ ] => destruct H
+               | _ => progress subst
+               | [ H : ~(_ \/ _) |- _ ] => apply Decidable.not_or in H
+               | [ H : _ /\ _ |- _ ] => destruct H
+               | [ H : ?x <> ?x |- _ ] => exfalso; apply (H eq_refl)
+               | _ => apply Lt.lt_n_S
+               | _ => apply Le.le_n_S
+               | _ => apply filter_list_dec
+               | [ H : _ -> _ -> ?G |- ?G ] => apply H; auto
+             end. }
+  Defined.
+  Lemma rdp_list_ntl_wf : well_founded rdp_list_productions_listT_R.
+  Proof.
+    unfold rdp_list_productions_listT_R.
+    intro.
+    apply well_founded_ltof.
+  Defined.
+End recursive_descent_parser_list.
+
+Section example_parse_string_grammar.
+  Fixpoint make_all_single_splits (str : string) : list { strs : string * string | (fst strs ++ snd strs = str)%string }.
+  Proof.
+    refine ((exist _ (""%string, str) eq_refl)::_).
+    refine (match str with
+              | ""%string => nil
+              | String.String ch str' => map (fun p => exist _ (String.String ch (fst (proj1_sig p)),
+                                                                snd (proj1_sig p))
+                                                             _)
+                                             (make_all_single_splits str')
+            end).
+    simpl; apply f_equal.
+    apply proj2_sig.
+  Defined.
+
+  Lemma length_append (s1 s2 : string) : length (s1 ++ s2) = length s1 + length s2.
+  Proof.
+    revert s2.
+    induction s1; simpl; trivial; [].
+    intros.
+    f_equal; auto.
+  Qed.
+
+  Fixpoint flatten1 {T} (ls : list (list T)) : list T
+    := match ls with
+         | nil => nil
+         | x::xs => (x ++ flatten1 xs)%list
+       end.
+
+  Lemma flatten1_length_ne_0 {T} (ls : list (list T)) (H0 : Datatypes.length ls <> 0)
+        (H1 : Datatypes.length (hd nil ls) <> 0)
+  : Datatypes.length (flatten1 ls) <> 0.
+  Proof.
+    destruct ls as [| [|] ]; simpl in *; auto.
+  Qed.
+
+  Local Ltac t' :=
+    match goal with
+      | _ => progress simpl in *
+      | _ => progress subst
+      | [ H : ?a = ?b |- _ ] => progress subst a
+      | [ H : ?a = ?b |- _ ] => progress subst b
+      | _ => rewrite (LeftId string_stringlike _)
+      | _ => rewrite (RightId string_stringlike _)
+      | _ => reflexivity
+      | _ => split
+      | _ => right; reflexivity
+      | _ => rewrite map_length
+      | _ => rewrite map_map
+      | _ => rewrite length_append
+      | _ => progress destruct_head_hnf prod
+      | _ => progress destruct_head_hnf and
+      | _ => progress destruct_head_hnf or
+      | _ => progress destruct_head_hnf sig
+      | _ => progress auto with arith
+      | _ => apply f_equal
+      | _ => solve [ apply proj2_sig ]
+      | _ => solve [ left; auto with arith ]
+      | [ str : string |- _ ] => solve [ destruct str; simpl; auto with arith ]
+      | [ str : string |- _ ] => solve [ left; destruct str; simpl; auto with arith ]
+    end.
+  Local Ltac t'' :=
+    match goal with
+      | _ => progress t'
+      | [ str : string |- _ ] => solve [ destruct str; repeat t' ]
+    end.
+  Local Ltac t :=
+    solve [ repeat t'' ].
+
+  Local Hint Resolve NPeano.Nat.lt_lt_add_l NPeano.Nat.lt_lt_add_r NPeano.Nat.lt_add_pos_r NPeano.Nat.lt_add_pos_l : arith.
+
+  Definition brute_force_splitter
+  : forall (str : string_stringlike) (pat : production Ascii.ascii),
+      list
+        (list
+           { str_part : string_stringlike |
+             Length string_stringlike str_part < Length string_stringlike str \/
+             str_part = str }).
+  Proof.
+    simpl.
+    intros str [|pat pats];
+      [ exact nil (** no patterns, no split (actually, we should never encounter this case *)
+      | ].
+    revert str.
+    induction pats; simpl in *; intros str.
+    { (** We only get one thing in the list *)
+      refine (((exist _ str _)::nil)::nil).
+      simpl; auto with arith. }
+    { pose (make_all_single_splits str) as single_splits.
+      pose proof (map (@proj1_sig _ _) single_splits).
+      refine (flatten1
+                (map (fun s1s2p =>
+                        map
+                          (fun split_list => ((exist _ (fst (proj1_sig s1s2p)) _)
+                                                ::(map (fun s => exist _ (proj1_sig s) _)
+                                                       split_list)))
+                          (IHpats (snd (proj1_sig s1s2p))))
+                     single_splits));
+        subst_body;
+        clear;
+        abstract t. }
+  Defined.
+
+  Variable G : grammar Ascii.ascii.
+  Variable all_productions : list (productions Ascii.ascii).
+
+  Definition brute_force_make_parse_of : @String Ascii.ascii string_stringlike
+                                         -> productions Ascii.ascii
+                                         -> bool.
+  Proof.
+    eapply (@parse_productions _ _ G)
+    with (productions_listT := rdp_list_productions_listT)
+           (is_valid_productions := rdp_list_is_valid_productions Ascii.ascii_dec)
+           (remove_productions := rdp_list_remove_productions Ascii.ascii_dec)
+           (productions_listT_R := rdp_list_productions_listT_R).
+    { intros; exact all_productions. }
+    { apply rdp_list_remove_productions_dec. }
+    { apply rdp_list_ntl_wf. }
+    { intros; apply brute_force_splitter; assumption. }
+  Defined.
+End example_parse_string_grammar.
+
+Module example_parse_empty_grammar.
+  Definition make_parse_of : forall (str : string)
+                                    (prods : productions Ascii.ascii),
+                               bool
+    := @brute_force_make_parse_of (trivial_grammar _) (map (Lookup (trivial_grammar _)) (""::nil)%string).
+
+
+
+  Definition parse : string -> bool
+    := fun str => make_parse_of str (trivial_grammar _).
+
+  Time Compute parse "".
+  Check eq_refl : true = parse "".
+  Time Compute parse "a".
+  Check eq_refl : false = parse "a".
+  Time Compute parse "aa".
+  Check eq_refl : false = parse "aa".
+End example_parse_empty_grammar.
+
+Section examples.
+  Section ab_star.
+
+    Fixpoint production_of_string (s : string) : production Ascii.ascii
+      := match s with
+           | EmptyString => nil
+           | String.String ch s' => (Terminal ch)::production_of_string s'
+         end.
+
+    Coercion production_of_string : string >-> production.
+
+    Definition ab_star_grammar : grammar Ascii.ascii :=
+      {| Top_name := "ab_star";
+         Lookup := fun s =>
+                     if string_dec s ""
+                     then nil::nil
+                     else if string_dec s "ab"
+                          then ("ab"%string : production _)::nil
+                          else if string_dec s "ab_star"
+                               then ((NonTerminal _ ""%string)::nil)
+                                      ::((NonTerminal _ "ab"%string)::(NonTerminal _ "ab_star")::nil)
+                                      ::nil
+                               else nil::nil |}.
+
+    Definition make_parse_of : forall (str : string)
+                                      (prods : productions Ascii.ascii),
+                                 bool
+      := @brute_force_make_parse_of ab_star_grammar (map (Lookup ab_star_grammar) (""::"ab"::"ab_star"::nil)%string).
+
+
+
+    Definition parse : string -> bool
+      := fun str => make_parse_of str ab_star_grammar.
+
+    Time Compute parse "".
+    Check eq_refl : parse "" = true.
+    Time Compute parse "a".
+    Check eq_refl : parse "a" = false.
+    Time Compute parse "ab".
+    Check eq_refl : parse "ab" = true.
+    Time Compute parse "aa".
+    Check eq_refl : parse "aa" = false.
+    Time Compute parse "ba".
+    Check eq_refl : parse "ba" = false.
+    Time Compute parse "aba".
+    Check eq_refl : parse "aba" = false.
+    Time Compute parse "abab".
+    Check eq_refl : parse "abab" = true.
+  (* For debugging: *)(*
+  Goal True.
+    pose proof (eq_refl (parse "abab")) as s.
+    unfold parse in s.
+    unfold make_parse_of in s.
+    unfold brute_force_make_parse_of in s.
+    cbv beta zeta delta [parse_productions] in s.
+    cbv beta zeta delta [parse_productions_or_abort] in s.
+    rewrite Init.Wf.Fix_eq in s.
+    Ltac do_compute_in c H :=
+      let c' := (eval compute in c) in
+      change c with c' in H.
+    do_compute_in (lt_dec (Length string_stringlike "abab"%string) (Length string_stringlike "abab"%string)) s.
+    change (if in_right then ?x else ?y) with y in s.
+    cbv beta zeta delta [rdp_list_is_valid_productions] in s.
+                       *)
+  End ab_star.
+End examples.
